@prefix : <https://open-manufacturing.org/ontologies/I4.0/param/> .
@prefix owl: <http://www.w3.org/2002/07/owl#> .
@prefix rdf: <http://www.w3.org/1999/02/22-rdf-syntax-ns#> .
@prefix xml: <http://www.w3.org/XML/1998/namespace> .
@prefix xsd: <http://www.w3.org/2001/XMLSchema#> .
@prefix rdfs: <http://www.w3.org/2000/01/rdf-schema#> .
@prefix dc: <http://purl.org/dc/elements/1.1/> .
@base <https://open-manufacturing.org/ontologies/I4.0/param/> .

<https://open-manufacturing.org/ontologies/I4.0/param> rdf:type owl:Ontology ;
                                                                dc:contributor "https://www.linkedin.com/in/ram-sashank-dinavahi-123296a0/" ;
                                                                dc:created "April 27th, 2022"@en ;
                                                                dc:creator "Piotr Janik (Intel), Denis Molin (Tera Data), Soufiane Ameziane (Tera Data)"@en ,
                                                                                                          "https://www.linkedin.com/in/dr-felix-l%C3%B6sch-0083294b/" ,
                                                                                                          "https://www.linkedin.com/in/dr-irlan-grangel-gonzalez/" ,
                                                                                                          "https://www.linkedin.com/in/fabio-massari-b63892/" ,
                                                                                                          "https://www.linkedin.com/in/marcel-keller-5591a174/" ,
                                                                                                          "https://www.linkedin.com/in/nico-wilhelm-5b306867/" ;
                                                                dc:modified "June 22nd, 2022"@en ;
                                                                dc:title "OMP I4.0 Core Information Model - Parameter Ontology"@en ;
                                                                rdfs:comment "This ontology models concepts and relationships to organize production parameters."@en ;
                                                                rdfs:label "OMP I4.0 Core Information Model - Parameter Ontology"@en ;
                                                                owl:versionInfo "1.0"@en .

#################################################################
#    Object Properties
#################################################################

###  https://open-manufacturing.org/ontologies/I4.0/param/hasParameter
:hasParameter rdf:type owl:ObjectProperty ;
              rdfs:domain :ParameterSpecification ;
              rdfs:range :Parameter ;
              rdfs:comment "Relationship between \"ParameterSpecification\" and \"Parameter\""@en ;
              rdfs:label "has parameter" ,
                         "has parameter"@en .


###  https://open-manufacturing.org/ontologies/I4.0/param/hasUnit
:hasUnit rdf:type owl:ObjectProperty ;
         rdfs:domain :Parameter ;
         rdfs:range <http://purl.oclc.org/NET/ssnx/qu/qu#Unit> ;
         rdfs:comment "Relationship between \"Parameter\" and \"Unit\""@en ;
         rdfs:label "has unit" ,
                    "has unit"@en .


###  https://open-manufacturing.org/ontologies/I4.0/param/isValueOf
:isValueOf rdf:type owl:ObjectProperty ;
           rdfs:domain :ParameterValue ;
           rdfs:range :Parameter ;
           rdfs:comment "Relationship between \"ParameterValue\" and \"Parameter\""@en ;
           rdfs:label "is value of" ,
                      "is value of"@en .


#################################################################
#    Data properties
#################################################################

###  https://open-manufacturing.org/ontologies/I4.0/param/paramDataType
:paramDataType rdf:type owl:DatatypeProperty ;
               rdfs:domain :Parameter ;
               rdfs:comment "Defines the data type of a parameter. Valid ranges are all xsd data types"@en ;
               rdfs:label "param datatype" ,
                          "param datatype"@en .


###  https://open-manufacturing.org/ontologies/I4.0/param/paramMaxTolerance
:paramMaxTolerance rdf:type owl:DatatypeProperty ;
                   rdfs:domain :Parameter ;
                   rdfs:comment "Defines the upper tolerance limit of a parameter."@en ;
                   rdfs:label "parameter max tolerance" ,
                              "parameter max tolerance"@en .


###  https://open-manufacturing.org/ontologies/I4.0/param/paramMinTolerance
:paramMinTolerance rdf:type owl:DatatypeProperty ;
                   rdfs:domain :Parameter ;
                   rdfs:comment "Defines the lower tolerance limit of a parameter."@en ;
                   rdfs:label "parameter min tolerance" ,
                              "parameter min tolerance"@en .


###  https://open-manufacturing.org/ontologies/I4.0/param/paramValue
:paramValue rdf:type owl:DatatypeProperty ;
            rdfs:domain :ParameterValue ;
            rdfs:comment "Defines the value of a parameter."@en ;
            rdfs:label "parameter value" ,
                       "parameter value"@en .


#################################################################
#    Classes
#################################################################

###  http://purl.oclc.org/NET/ssnx/qu/qu#Unit
<http://purl.oclc.org/NET/ssnx/qu/qu#Unit> rdf:type owl:Class .


###  https://open-manufacturing.org/ontologies/I4.0/param/Parameter
:Parameter rdf:type owl:Class ;
           rdfs:subClassOf owl:Thing ;
           rdfs:comment "An individually measured item or property of a process segment or product segment. Parameters belong to a Parameter Specification."@en ;
           rdfs:label "Parameter" ,
                      "Parameter"@en .


###  https://open-manufacturing.org/ontologies/I4.0/param/ParameterSpecification
:ParameterSpecification rdf:type owl:Class ;
                        rdfs:subClassOf owl:Thing ;
                        rdfs:comment "Specifies the setting parameters and/or result parameters for a process segment or product segment. A parameter specification consists of 1..n parameters."@en ;
                        rdfs:label "Parameter Specification" ,
                                   "Parameter Specification"@en .


###  https://open-manufacturing.org/ontologies/I4.0/param/ParameterValue
:ParameterValue rdf:type owl:Class ;
                rdfs:subClassOf owl:Thing ;
                rdfs:comment """Concrete value of a parameter.
Note 1: For example, the parameter value of the parameter “Temperature” might be “18.5”."""@en ;
                rdfs:label "Parameter Value" ,
                           "Parameter Value"@en .


###  https://open-manufacturing.org/ontologies/I4.0/param/ResultParameter
:ResultParameter rdf:type owl:Class ;
                 rdfs:subClassOf :Parameter ;
                 rdfs:comment "Description of the result parameters of a given process or product segment. Result parameters can also contain tolerance values. Subclass of Parameter"@en ;
                 rdfs:label "Result Parameter" ,
                            "Result Parameter"@en .


###  https://open-manufacturing.org/ontologies/I4.0/param/SettingParameter
:SettingParameter rdf:type owl:Class ;
                  rdfs:subClassOf :Parameter ;
                  rdfs:comment """Description of input / setting parameters of a given process or product segment. Subclass of Parameter.
Note 1: Setting parameters can also contain tolerance values."""@en ;
                  rdfs:label "Setting Parameter" ,
                             "Setting Parameter"@en .


###  Generated by the OWL API (version 4.5.9.2019-02-01T07:24:44Z) https://github.com/owlcs/owlapi
