<?xml version="1.0"?>
<rdf:RDF xmlns="https://open-manufacturing.org/ontologies/I4.0/Core#"
     xml:base="https://open-manufacturing.org/ontologies/I4.0/Core"
     xmlns:dc="http://purl.org/dc/elements/1.1/"
     xmlns:owl="http://www.w3.org/2002/07/owl#"
     xmlns:rdf="http://www.w3.org/1999/02/22-rdf-syntax-ns#"
     xmlns:xml="http://www.w3.org/XML/1998/namespace"
     xmlns:xsd="http://www.w3.org/2001/XMLSchema#"
     xmlns:rdfs="http://www.w3.org/2000/01/rdf-schema#">
    <owl:Ontology rdf:about="https://open-manufacturing.org/ontologies/I4.0/Core">
        <owl:imports rdf:resource="https://open-manufacturing.org/ontologies/I4.0/Equipment"/>
        <owl:imports rdf:resource="https://open-manufacturing.org/ontologies/I4.0/Parameter"/>
        <owl:imports rdf:resource="https://open-manufacturing.org/ontologies/I4.0/PhysicalAsset"/>
        <owl:imports rdf:resource="https://open-manufacturing.org/ontologies/I4.0/Product"/>
        <owl:imports rdf:resource="https://open-manufacturing.org/ontologies/I4.0/processsegment"/>
        <owl:imports rdf:resource="https://open-manufacturing.org/ontologies/I4.0/ProductSegment/"/>
        <dc:created xml:lang="en">July 13th, 2022</dc:created>
        <dc:creator xml:lang="en">Irlan Grangel-Gonzalez, Felix Loesch</dc:creator>
        <dc:creator>https://www.linkedin.com/in/dr-felix-l%C3%B6sch-0083294b/</dc:creator>
        <dc:creator>https://www.linkedin.com/in/dr-irlan-grangel-gonzalez/</dc:creator>
        <dc:creator>https://www.linkedin.com/in/fabio-massari-b63892/</dc:creator>
        <dc:creator>https://www.linkedin.com/in/marcel-keller-5591a174/</dc:creator>
        <dc:creator>https://www.linkedin.com/in/nico-wilhelm-5b306867/</dc:creator>
        <dc:modified xml:lang="en">July 18th, 2022</dc:modified>
        <dc:title xml:lang="en">OMP I4.0 Core Information Model - Core Ontology</dc:title>
        <rdfs:comment xml:lang="en">The OMP I4.0 Core Information Model provides a common and standardized definition of relevant manufacturing entities, their attributes, and relationships, including their semantic meaning. The contents of the information model are based on the IEC 62264-1 standard. The Information model is implemented in a set of modularized ontologies. This enables manufacturing enterprises to efficiently integrate data and provide a clear semantic context, thus reducing the time required to generate insights from the data. Furthermore, the OMP I4.0 Core Information Model allows companies to reuse data-processing applications across heterogeneous data sources as the standardized data model acts as an abstraction layer over the heterogeneous data decoupling data sources from data processing applications.</rdfs:comment>
        <rdfs:label xml:lang="en">OMP I4.0 Core Information Model - Core Ontology</rdfs:label>
        <owl:versionInfo xml:lang="en">1.0</owl:versionInfo>
    </owl:Ontology>
    


    <!-- 
    ///////////////////////////////////////////////////////////////////////////////////////
    //
    // Annotation properties
    //
    ///////////////////////////////////////////////////////////////////////////////////////
     -->


    


    <!-- http://purl.org/dc/elements/1.1/created -->


    <owl:AnnotationProperty rdf:about="http://purl.org/dc/elements/1.1/created"/>
    


    <!-- http://purl.org/dc/elements/1.1/creator -->


    <owl:AnnotationProperty rdf:about="http://purl.org/dc/elements/1.1/creator"/>
    


    <!-- http://purl.org/dc/elements/1.1/modified -->


    <owl:AnnotationProperty rdf:about="http://purl.org/dc/elements/1.1/modified"/>
    


    <!-- http://purl.org/dc/elements/1.1/title -->


    <owl:AnnotationProperty rdf:about="http://purl.org/dc/elements/1.1/title"/>
    


    <!-- 
    ///////////////////////////////////////////////////////////////////////////////////////
    //
    // Object Properties
    //
    ///////////////////////////////////////////////////////////////////////////////////////
     -->


    


    <!-- https://open-manufacturing.org/ontologies/I4.0/Core/hasEquipment -->


    <owl:ObjectProperty rdf:about="https://open-manufacturing.org/ontologies/I4.0/Core/hasEquipment">
        <rdfs:domain rdf:resource="https://open-manufacturing.org/ontologies/I4.0/ProductSegment/EquipmentSpecification"/>
        <rdfs:range rdf:resource="https://open-manufacturing.org/ontologies/I4.0/Equipment/Equipment"/>
        <rdfs:comment xml:lang="en">Relationship between &quot;EquipmentSpecification&quot; and &quot;Equipment&quot;</rdfs:comment>
        <rdfs:label>has equipment</rdfs:label>
    </owl:ObjectProperty>
    


    <!-- https://open-manufacturing.org/ontologies/I4.0/Core/hasMaterial -->


    <owl:ObjectProperty rdf:about="https://open-manufacturing.org/ontologies/I4.0/Core/hasMaterial">
        <rdfs:domain rdf:resource="https://open-manufacturing.org/ontologies/I4.0/ProductSegment/MaterialSpecification"/>
        <rdfs:range rdf:resource="https://open-manufacturing.org/ontologies/I4.0/Product/Material"/>
        <rdfs:comment xml:lang="en">Relationship between &quot;MaterialSpecification&quot; and &quot;Material&quot;</rdfs:comment>
        <rdfs:label>has material</rdfs:label>
    </owl:ObjectProperty>
    


    <!-- https://open-manufacturing.org/ontologies/I4.0/Core/hasParameterSpecification -->


    <owl:ObjectProperty rdf:about="https://open-manufacturing.org/ontologies/I4.0/Core/hasParameterSpecification">
        <rdfs:subPropertyOf rdf:resource="http://www.w3.org/2002/07/owl#topObjectProperty"/>
        <rdfs:domain rdf:resource="https://open-manufacturing.org/ontologies/I4.0/ProcessSegment/ProcessSegment"/>
        <rdfs:domain rdf:resource="https://open-manufacturing.org/ontologies/I4.0/ProductSegment/ProductSegment"/>
        <rdfs:range rdf:resource="https://open-manufacturing.org/ontologies/I4.0/Parameter/ParameterSpecification"/>
        <rdfs:comment xml:lang="en">Relationship between &quot;ProcessSegment&quot; and &quot;ProductSegment&quot;</rdfs:comment>
        <rdfs:label>has parameter specification</rdfs:label>
    </owl:ObjectProperty>
    


    <!-- https://open-manufacturing.org/ontologies/I4.0/Core/hasParameterValue -->


    <owl:ObjectProperty rdf:about="https://open-manufacturing.org/ontologies/I4.0/Core/hasParameterValue">
        <rdfs:domain rdf:resource="https://open-manufacturing.org/ontologies/I4.0/ProductSegment/SegmentResult"/>
        <rdfs:range rdf:resource="https://open-manufacturing.org/ontologies/I4.0/Parameter/ParameterValue"/>
        <rdfs:comment xml:lang="en">Relationship between &quot;SegmentResult&quot; and &quot;ParameterValue&quot;</rdfs:comment>
        <rdfs:label>has parameter value</rdfs:label>
    </owl:ObjectProperty>
    


    <!-- https://open-manufacturing.org/ontologies/I4.0/Core/implementsProcessSegment -->


    <owl:ObjectProperty rdf:about="https://open-manufacturing.org/ontologies/I4.0/Core/implementsProcessSegment">
        <rdfs:domain rdf:resource="https://open-manufacturing.org/ontologies/I4.0/ProductSegment/ProductSegment"/>
        <rdfs:range rdf:resource="https://open-manufacturing.org/ontologies/I4.0/ProcessSegment/ProcessSegment"/>
        <rdfs:comment xml:lang="en">Relationship between &quot;ProductSegment&quot; and &quot;ProcessSegment&quot;</rdfs:comment>
        <rdfs:label>implements process segment</rdfs:label>
    </owl:ObjectProperty>
    


    <!-- https://open-manufacturing.org/ontologies/I4.0/Core/isImplementedByAsset -->


    <owl:ObjectProperty rdf:about="https://open-manufacturing.org/ontologies/I4.0/Core/isImplementedByAsset">
        <rdfs:domain rdf:resource="https://open-manufacturing.org/ontologies/I4.0/Equipment/WorkUnit"/>
        <rdfs:range rdf:resource="https://open-manufacturing.org/ontologies/I4.0/PhysicalAsset/Asset"/>
        <rdfs:comment xml:lang="en">Relationship between &quot;WorkUnit&quot; and &quot;Asset&quot;</rdfs:comment>
        <rdfs:label>is implemented by asset</rdfs:label>
    </owl:ObjectProperty>
    


    <!-- https://open-manufacturing.org/ontologies/I4.0/Core/requiresProductSegment -->


    <owl:ObjectProperty rdf:about="https://open-manufacturing.org/ontologies/I4.0/Core/requiresProductSegment">
        <rdfs:domain rdf:resource="https://open-manufacturing.org/ontologies/I4.0/Product/Product"/>
        <rdfs:range rdf:resource="https://open-manufacturing.org/ontologies/I4.0/ProductSegment/ProductSegment"/>
        <rdfs:comment xml:lang="en">Relationship between &quot;Product&quot; and &quot;ProductSegment&quot;</rdfs:comment>
        <rdfs:label>requires product segment</rdfs:label>
    </owl:ObjectProperty>
    


    <!-- https://open-manufacturing.org/ontologies/I4.0/Equipment/belongsToLine -->


    <owl:ObjectProperty rdf:about="https://open-manufacturing.org/ontologies/I4.0/Equipment/belongsToLine">
        <rdfs:subPropertyOf rdf:resource="http://www.w3.org/2002/07/owl#topObjectProperty"/>
        <rdfs:domain rdf:resource="https://open-manufacturing.org/ontologies/I4.0/Equipment/Station"/>
        <rdfs:range rdf:resource="https://open-manufacturing.org/ontologies/I4.0/Equipment/Line"/>
        <rdfs:label xml:lang="en">belongs to line</rdfs:label>
    </owl:ObjectProperty>
    


    <!-- https://open-manufacturing.org/ontologies/I4.0/Equipment/belongsToPlant -->


    <owl:ObjectProperty rdf:about="https://open-manufacturing.org/ontologies/I4.0/Equipment/belongsToPlant">
        <rdfs:subPropertyOf rdf:resource="http://www.w3.org/2002/07/owl#topObjectProperty"/>
        <rdfs:domain rdf:resource="https://open-manufacturing.org/ontologies/I4.0/Equipment/WorkCenter"/>
        <rdfs:range rdf:resource="https://open-manufacturing.org/ontologies/I4.0/Equipment/Plant"/>
        <rdfs:comment xml:lang="en">Relationship between &quot;WorkCenter&quot; and &quot;Plant&quot;</rdfs:comment>
        <rdfs:label xml:lang="en">belongs to plant</rdfs:label>
    </owl:ObjectProperty>
    


    <!-- https://open-manufacturing.org/ontologies/I4.0/Equipment/belongsToStation -->


    <owl:ObjectProperty rdf:about="https://open-manufacturing.org/ontologies/I4.0/Equipment/belongsToStation">
        <rdfs:subPropertyOf rdf:resource="http://www.w3.org/2002/07/owl#topObjectProperty"/>
        <rdfs:domain rdf:resource="https://open-manufacturing.org/ontologies/I4.0/Equipment/WorkCell"/>
        <rdfs:range rdf:resource="https://open-manufacturing.org/ontologies/I4.0/Equipment/Station"/>
        <rdfs:comment xml:lang="en">Relationship between &quot;WorkCell&quot; and &quot;Station&quot;</rdfs:comment>
        <rdfs:label xml:lang="en">belongs to station</rdfs:label>
    </owl:ObjectProperty>
    


    <!-- https://open-manufacturing.org/ontologies/I4.0/Equipment/belongsToWorkCenter -->


    <owl:ObjectProperty rdf:about="https://open-manufacturing.org/ontologies/I4.0/Equipment/belongsToWorkCenter">
        <rdfs:subPropertyOf rdf:resource="http://www.w3.org/2002/07/owl#topObjectProperty"/>
        <rdfs:domain rdf:resource="https://open-manufacturing.org/ontologies/I4.0/Equipment/WorkUnit"/>
        <rdfs:range rdf:resource="https://open-manufacturing.org/ontologies/I4.0/Equipment/WorkCenter"/>
        <rdfs:comment xml:lang="en">Relationship between &quot;WorkUnit&quot; and &quot;WorkCenter&quot;</rdfs:comment>
        <rdfs:label xml:lang="en">belongs to work center</rdfs:label>
    </owl:ObjectProperty>
    


    <!-- https://open-manufacturing.org/ontologies/I4.0/Equipment/consistsOfStation -->


    <owl:ObjectProperty rdf:about="https://open-manufacturing.org/ontologies/I4.0/Equipment/consistsOfStation">
        <rdfs:subPropertyOf rdf:resource="http://www.w3.org/2002/07/owl#topObjectProperty"/>
        <rdfs:domain rdf:resource="https://open-manufacturing.org/ontologies/I4.0/Equipment/Line"/>
        <rdfs:range rdf:resource="https://open-manufacturing.org/ontologies/I4.0/Equipment/Station"/>
        <rdfs:comment xml:lang="en">Relationship between &quot;Line&quot; and &quot;Station&quot;</rdfs:comment>
        <rdfs:label xml:lang="en">consists of station</rdfs:label>
    </owl:ObjectProperty>
    


    <!-- https://open-manufacturing.org/ontologies/I4.0/Equipment/consistsOfWorkCell -->


    <owl:ObjectProperty rdf:about="https://open-manufacturing.org/ontologies/I4.0/Equipment/consistsOfWorkCell">
        <rdfs:subPropertyOf rdf:resource="http://www.w3.org/2002/07/owl#topObjectProperty"/>
        <rdfs:domain rdf:resource="https://open-manufacturing.org/ontologies/I4.0/Equipment/Station"/>
        <rdfs:range rdf:resource="https://open-manufacturing.org/ontologies/I4.0/Equipment/WorkCell"/>
        <rdfs:comment xml:lang="en">Relationship between &quot;Station&quot; and &quot;WorkCell&quot;</rdfs:comment>
        <rdfs:label xml:lang="en">consists of work cell</rdfs:label>
    </owl:ObjectProperty>
    


    <!-- https://open-manufacturing.org/ontologies/I4.0/Equipment/consistsOfWorkCenter -->


    <owl:ObjectProperty rdf:about="https://open-manufacturing.org/ontologies/I4.0/Equipment/consistsOfWorkCenter">
        <rdfs:subPropertyOf rdf:resource="http://www.w3.org/2002/07/owl#topObjectProperty"/>
        <rdfs:domain rdf:resource="https://open-manufacturing.org/ontologies/I4.0/Equipment/Plant"/>
        <rdfs:range rdf:resource="https://open-manufacturing.org/ontologies/I4.0/Equipment/WorkCenter"/>
        <rdfs:comment xml:lang="en">Relationship between &quot;Plant&quot; and &quot;WorkCenter&quot;</rdfs:comment>
        <rdfs:label xml:lang="en">consists of work center</rdfs:label>
    </owl:ObjectProperty>
    


    <!-- https://open-manufacturing.org/ontologies/I4.0/Equipment/consistsOfWorkUnit -->


    <owl:ObjectProperty rdf:about="https://open-manufacturing.org/ontologies/I4.0/Equipment/consistsOfWorkUnit">
        <rdfs:subPropertyOf rdf:resource="http://www.w3.org/2002/07/owl#topObjectProperty"/>
        <rdfs:domain rdf:resource="https://open-manufacturing.org/ontologies/I4.0/Equipment/WorkCenter"/>
        <rdfs:range rdf:resource="https://open-manufacturing.org/ontologies/I4.0/Equipment/WorkUnit"/>
        <rdfs:comment xml:lang="en">Relationship between &quot;WorkCenter&quot; and &quot;WorkUnit&quot;</rdfs:comment>
        <rdfs:label xml:lang="en">consists of work unit</rdfs:label>
    </owl:ObjectProperty>
    


    <!-- https://open-manufacturing.org/ontologies/I4.0/Equipment/madeUpOfWorkUnit -->


    <owl:ObjectProperty rdf:about="https://open-manufacturing.org/ontologies/I4.0/Equipment/madeUpOfWorkUnit">
        <rdfs:subPropertyOf rdf:resource="http://www.w3.org/2002/07/owl#topObjectProperty"/>
        <rdfs:domain rdf:resource="https://open-manufacturing.org/ontologies/I4.0/Equipment/WorkUnit"/>
        <rdfs:range rdf:resource="https://open-manufacturing.org/ontologies/I4.0/Equipment/WorkUnit"/>
        <rdfs:comment xml:lang="en">Transitive Relationship between &quot;WorkUnit&quot; with itself</rdfs:comment>
        <rdfs:label xml:lang="en">made up of work unit</rdfs:label>
    </owl:ObjectProperty>
    


    <!-- https://open-manufacturing.org/ontologies/I4.0/Parameter/hasParameter -->


    <owl:ObjectProperty rdf:about="https://open-manufacturing.org/ontologies/I4.0/Parameter/hasParameter">
        <rdfs:domain rdf:resource="https://open-manufacturing.org/ontologies/I4.0/Parameter/ParameterSpecification"/>
        <rdfs:range rdf:resource="https://open-manufacturing.org/ontologies/I4.0/Parameter/Parameter"/>
        <rdfs:comment xml:lang="en">Relationship between &quot;ParameterSpecification&quot; and &quot;Parameter&quot;</rdfs:comment>
        <rdfs:label xml:lang="en">has parameter</rdfs:label>
        <rdfs:label>has parameter</rdfs:label>
    </owl:ObjectProperty>
    


    <!-- https://open-manufacturing.org/ontologies/I4.0/Parameter/hasUnit -->


    <owl:ObjectProperty rdf:about="https://open-manufacturing.org/ontologies/I4.0/Parameter/hasUnit">
        <rdfs:domain rdf:resource="https://open-manufacturing.org/ontologies/I4.0/Parameter/Parameter"/>
        <rdfs:range rdf:resource="http://purl.oclc.org/NET/ssnx/qu/qu#Unit"/>
        <rdfs:comment xml:lang="en">Relationship between &quot;Parameter&quot; and &quot;Unit&quot;</rdfs:comment>
        <rdfs:label xml:lang="en">has unit</rdfs:label>
        <rdfs:label>has unit</rdfs:label>
    </owl:ObjectProperty>
    


    <!-- https://open-manufacturing.org/ontologies/I4.0/Parameter/isValueOf -->


    <owl:ObjectProperty rdf:about="https://open-manufacturing.org/ontologies/I4.0/Parameter/isValueOf">
        <rdfs:domain rdf:resource="https://open-manufacturing.org/ontologies/I4.0/Parameter/ParameterValue"/>
        <rdfs:range rdf:resource="https://open-manufacturing.org/ontologies/I4.0/Parameter/Parameter"/>
        <rdfs:comment xml:lang="en">Relationship between &quot;ParameterValue&quot; and &quot;Parameter&quot;</rdfs:comment>
        <rdfs:label xml:lang="en">is value of</rdfs:label>
        <rdfs:label>is value of</rdfs:label>
    </owl:ObjectProperty>
    


    <!-- https://open-manufacturing.org/ontologies/I4.0/PhysicalAsset/belongsToBuilding -->


    <owl:ObjectProperty rdf:about="https://open-manufacturing.org/ontologies/I4.0/PhysicalAsset/belongsToBuilding">
        <rdfs:domain rdf:resource="https://open-manufacturing.org/ontologies/I4.0/PhysicalAsset/Level"/>
        <rdfs:range rdf:resource="https://open-manufacturing.org/ontologies/I4.0/PhysicalAsset/Building"/>
        <rdfs:label xml:lang="en">belongs to building</rdfs:label>
    </owl:ObjectProperty>
    


    <!-- https://open-manufacturing.org/ontologies/I4.0/PhysicalAsset/belongsToLocation -->


    <owl:ObjectProperty rdf:about="https://open-manufacturing.org/ontologies/I4.0/PhysicalAsset/belongsToLocation">
        <rdfs:domain rdf:resource="https://open-manufacturing.org/ontologies/I4.0/PhysicalAsset/Building"/>
        <rdfs:range rdf:resource="https://open-manufacturing.org/ontologies/I4.0/PhysicalAsset/Location"/>
        <rdfs:label xml:lang="en">belongs to location</rdfs:label>
    </owl:ObjectProperty>
    


    <!-- https://open-manufacturing.org/ontologies/I4.0/PhysicalAsset/belongsToMachine -->


    <owl:ObjectProperty rdf:about="https://open-manufacturing.org/ontologies/I4.0/PhysicalAsset/belongsToMachine">
        <rdfs:domain rdf:resource="https://open-manufacturing.org/ontologies/I4.0/PhysicalAsset/MachineComponent"/>
        <rdfs:range rdf:resource="https://open-manufacturing.org/ontologies/I4.0/PhysicalAsset/Machine"/>
        <rdfs:label xml:lang="en">belongs to machine</rdfs:label>
    </owl:ObjectProperty>
    


    <!-- https://open-manufacturing.org/ontologies/I4.0/PhysicalAsset/consistsOfBuilding -->


    <owl:ObjectProperty rdf:about="https://open-manufacturing.org/ontologies/I4.0/PhysicalAsset/consistsOfBuilding">
        <rdfs:domain rdf:resource="https://open-manufacturing.org/ontologies/I4.0/PhysicalAsset/Location"/>
        <rdfs:range rdf:resource="https://open-manufacturing.org/ontologies/I4.0/PhysicalAsset/Building"/>
        <rdfs:label xml:lang="en">consists of building</rdfs:label>
    </owl:ObjectProperty>
    


    <!-- https://open-manufacturing.org/ontologies/I4.0/PhysicalAsset/consistsOfLevel -->


    <owl:ObjectProperty rdf:about="https://open-manufacturing.org/ontologies/I4.0/PhysicalAsset/consistsOfLevel">
        <rdfs:domain rdf:resource="https://open-manufacturing.org/ontologies/I4.0/PhysicalAsset/Building"/>
        <rdfs:range rdf:resource="https://open-manufacturing.org/ontologies/I4.0/PhysicalAsset/Level"/>
        <rdfs:label xml:lang="en">consists of level</rdfs:label>
    </owl:ObjectProperty>
    


    <!-- https://open-manufacturing.org/ontologies/I4.0/PhysicalAsset/consistsOfMachineComponent -->


    <owl:ObjectProperty rdf:about="https://open-manufacturing.org/ontologies/I4.0/PhysicalAsset/consistsOfMachineComponent">
        <rdfs:domain rdf:resource="https://open-manufacturing.org/ontologies/I4.0/PhysicalAsset/Machine"/>
        <rdfs:range rdf:resource="https://open-manufacturing.org/ontologies/I4.0/PhysicalAsset/MachineComponent"/>
        <rdfs:label xml:lang="en">consists of machine component</rdfs:label>
    </owl:ObjectProperty>
    


    <!-- https://open-manufacturing.org/ontologies/I4.0/PhysicalAsset/hasPhysicalAsset -->


    <owl:ObjectProperty rdf:about="https://open-manufacturing.org/ontologies/I4.0/PhysicalAsset/hasPhysicalAsset">
        <rdfs:domain rdf:resource="https://open-manufacturing.org/ontologies/I4.0/PhysicalAsset/Building"/>
        <rdfs:range rdf:resource="https://open-manufacturing.org/ontologies/I4.0/PhysicalAsset/Asset"/>
        <rdfs:label xml:lang="en">has physical asset</rdfs:label>
    </owl:ObjectProperty>
    


    <!-- https://open-manufacturing.org/ontologies/I4.0/PhysicalAsset/isComposedOfMachineComponent -->


    <owl:ObjectProperty rdf:about="https://open-manufacturing.org/ontologies/I4.0/PhysicalAsset/isComposedOfMachineComponent">
        <rdfs:domain rdf:resource="https://open-manufacturing.org/ontologies/I4.0/PhysicalAsset/MachineComponent"/>
        <rdfs:range rdf:resource="https://open-manufacturing.org/ontologies/I4.0/PhysicalAsset/MachineComponent"/>
        <rdfs:label xml:lang="en">is composed of machine component</rdfs:label>
    </owl:ObjectProperty>
    


    <!-- https://open-manufacturing.org/ontologies/I4.0/PhysicalAsset/isLocatedInBuilding -->


    <owl:ObjectProperty rdf:about="https://open-manufacturing.org/ontologies/I4.0/PhysicalAsset/isLocatedInBuilding">
        <rdfs:domain rdf:resource="https://open-manufacturing.org/ontologies/I4.0/PhysicalAsset/Asset"/>
        <rdfs:range rdf:resource="https://open-manufacturing.org/ontologies/I4.0/PhysicalAsset/Building"/>
        <rdfs:label xml:lang="en">is located in building</rdfs:label>
    </owl:ObjectProperty>
    


    <!-- https://open-manufacturing.org/ontologies/I4.0/PhysicalAsset/isUsedByMachineComponent -->


    <owl:ObjectProperty rdf:about="https://open-manufacturing.org/ontologies/I4.0/PhysicalAsset/isUsedByMachineComponent">
        <rdfs:domain rdf:resource="https://open-manufacturing.org/ontologies/I4.0/PhysicalAsset/MachineTool"/>
        <rdfs:range rdf:resource="https://open-manufacturing.org/ontologies/I4.0/PhysicalAsset/MachineComponent"/>
        <rdfs:label xml:lang="en">is used by machine component</rdfs:label>
    </owl:ObjectProperty>
    


    <!-- https://open-manufacturing.org/ontologies/I4.0/PhysicalAsset/usesMachineTool -->


    <owl:ObjectProperty rdf:about="https://open-manufacturing.org/ontologies/I4.0/PhysicalAsset/usesMachineTool">
        <rdfs:domain rdf:resource="https://open-manufacturing.org/ontologies/I4.0/PhysicalAsset/MachineComponent"/>
        <rdfs:range rdf:resource="https://open-manufacturing.org/ontologies/I4.0/PhysicalAsset/MachineTool"/>
        <rdfs:label xml:lang="en">uses machine tool</rdfs:label>
    </owl:ObjectProperty>
    


    <!-- https://open-manufacturing.org/ontologies/I4.0/ProcessSegment/belongsToProcess -->


    <owl:ObjectProperty rdf:about="https://open-manufacturing.org/ontologies/I4.0/ProcessSegment/belongsToProcess">
        <rdfs:domain rdf:resource="https://open-manufacturing.org/ontologies/I4.0/ProcessSegment/ProcessSegment"/>
        <rdfs:range rdf:resource="https://open-manufacturing.org/ontologies/I4.0/ProcessSegment/Process"/>
        <rdfs:label xml:lang="en">belongs to process</rdfs:label>
        <rdfs:label>belongs to process</rdfs:label>
    </owl:ObjectProperty>
    


    <!-- https://open-manufacturing.org/ontologies/I4.0/ProcessSegment/consistsOfProcessSegment -->


    <owl:ObjectProperty rdf:about="https://open-manufacturing.org/ontologies/I4.0/ProcessSegment/consistsOfProcessSegment">
        <rdfs:domain rdf:resource="https://open-manufacturing.org/ontologies/I4.0/ProcessSegment/Process"/>
        <rdfs:range rdf:resource="https://open-manufacturing.org/ontologies/I4.0/ProcessSegment/ProcessSegment"/>
        <rdfs:label xml:lang="en">consists of process segment</rdfs:label>
        <rdfs:label>consists of process segment</rdfs:label>
    </owl:ObjectProperty>
    


    <!-- https://open-manufacturing.org/ontologies/I4.0/Product/assembledFromMaterial -->


    <owl:ObjectProperty rdf:about="https://open-manufacturing.org/ontologies/I4.0/Product/assembledFromMaterial">
        <rdfs:domain rdf:resource="https://open-manufacturing.org/ontologies/I4.0/Product/Material"/>
        <rdfs:range rdf:resource="https://open-manufacturing.org/ontologies/I4.0/Product/Material"/>
        <rdfs:label>assembled from material</rdfs:label>
    </owl:ObjectProperty>
    


    <!-- https://open-manufacturing.org/ontologies/I4.0/Product/assembledFromProcessedPart -->


    <owl:ObjectProperty rdf:about="https://open-manufacturing.org/ontologies/I4.0/Product/assembledFromProcessedPart">
        <rdfs:domain rdf:resource="https://open-manufacturing.org/ontologies/I4.0/Product/ProcessedPart"/>
        <rdfs:range rdf:resource="https://open-manufacturing.org/ontologies/I4.0/Product/ProcessedPart"/>
        <rdfs:label>assembled from processed part</rdfs:label>
    </owl:ObjectProperty>
    


    <!-- https://open-manufacturing.org/ontologies/I4.0/Product/relatesToMaterial -->


    <owl:ObjectProperty rdf:about="https://open-manufacturing.org/ontologies/I4.0/Product/relatesToMaterial">
        <rdfs:domain rdf:resource="https://open-manufacturing.org/ontologies/I4.0/Product/ProcessedPart"/>
        <rdfs:range rdf:resource="https://open-manufacturing.org/ontologies/I4.0/Product/Material"/>
        <rdfs:label>relates to material</rdfs:label>
    </owl:ObjectProperty>
    


    <!-- https://open-manufacturing.org/ontologies/I4.0/ProductSegment/hasEquipmentSpecification -->


    <owl:ObjectProperty rdf:about="https://open-manufacturing.org/ontologies/I4.0/ProductSegment/hasEquipmentSpecification">
        <rdfs:domain rdf:resource="https://open-manufacturing.org/ontologies/I4.0/ProductSegment/ProductSegment"/>
        <rdfs:range rdf:resource="https://open-manufacturing.org/ontologies/I4.0/ProductSegment/EquipmentSpecification"/>
        <rdfs:comment xml:lang="en">Relationship between &quot;ProductSegment&quot; and &quot;EquipmentSpecification&quot;</rdfs:comment>
        <rdfs:label xml:lang="en">has equipment specification</rdfs:label>
        <rdfs:label>has equipment specification</rdfs:label>
    </owl:ObjectProperty>
    


    <!-- https://open-manufacturing.org/ontologies/I4.0/ProductSegment/hasMaterialSpecification -->


    <owl:ObjectProperty rdf:about="https://open-manufacturing.org/ontologies/I4.0/ProductSegment/hasMaterialSpecification">
        <rdfs:domain rdf:resource="https://open-manufacturing.org/ontologies/I4.0/ProductSegment/ProductSegment"/>
        <rdfs:range rdf:resource="https://open-manufacturing.org/ontologies/I4.0/ProductSegment/MaterialSpecification"/>
        <rdfs:comment xml:lang="en">Relationship between &quot;ProductSegment&quot; and &quot;MaterialSpecification&quot;</rdfs:comment>
        <rdfs:label xml:lang="en">has material specification</rdfs:label>
        <rdfs:label>has material specification</rdfs:label>
    </owl:ObjectProperty>
    


    <!-- https://open-manufacturing.org/ontologies/I4.0/ProductSegment/hasSegmentResult -->


    <owl:ObjectProperty rdf:about="https://open-manufacturing.org/ontologies/I4.0/ProductSegment/hasSegmentResult">
        <rdfs:domain rdf:resource="https://open-manufacturing.org/ontologies/I4.0/ProductSegment/ProductSegment"/>
        <rdfs:range rdf:resource="https://open-manufacturing.org/ontologies/I4.0/ProductSegment/SegmentResult"/>
        <rdfs:comment xml:lang="en">Relationship between &quot;ProductSegment&quot; and &quot;SegmentResult&quot;</rdfs:comment>
        <rdfs:label xml:lang="en">has segment result</rdfs:label>
        <rdfs:label>has segment result</rdfs:label>
    </owl:ObjectProperty>
    


    <!-- https://open-manufacturing.org/ontologies/I4.0/ProductSegment/isFollowedBy -->


    <owl:ObjectProperty rdf:about="https://open-manufacturing.org/ontologies/I4.0/ProductSegment/isFollowedBy">
        <rdfs:domain rdf:resource="https://open-manufacturing.org/ontologies/I4.0/ProductSegment/ProductSegment"/>
        <rdfs:range rdf:resource="https://open-manufacturing.org/ontologies/I4.0/ProductSegment/ProductSegment"/>
        <rdfs:comment xml:lang="en">Relationship between &quot;ProductSegment&quot; and &quot;ProductSegment&quot;</rdfs:comment>
        <rdfs:label xml:lang="en">is followed by</rdfs:label>
        <rdfs:label>is followed by</rdfs:label>
    </owl:ObjectProperty>
    


    <!-- 
    ///////////////////////////////////////////////////////////////////////////////////////
    //
    // Data properties
    //
    ///////////////////////////////////////////////////////////////////////////////////////
     -->


    


    <!-- https://open-manufacturing.org/ontologies/I4.0/Parameter/paramDataType -->


    <owl:DatatypeProperty rdf:about="https://open-manufacturing.org/ontologies/I4.0/Parameter/paramDataType">
        <rdfs:domain rdf:resource="https://open-manufacturing.org/ontologies/I4.0/Parameter/Parameter"/>
        <rdfs:comment xml:lang="en">Defines the data type of a parameter. Valid ranges are all xsd data types</rdfs:comment>
        <rdfs:label xml:lang="en">param datatype</rdfs:label>
        <rdfs:label>param datatype</rdfs:label>
    </owl:DatatypeProperty>
    


    <!-- https://open-manufacturing.org/ontologies/I4.0/Parameter/paramMaxTolerance -->


    <owl:DatatypeProperty rdf:about="https://open-manufacturing.org/ontologies/I4.0/Parameter/paramMaxTolerance">
        <rdfs:domain rdf:resource="https://open-manufacturing.org/ontologies/I4.0/Parameter/Parameter"/>
        <rdfs:comment xml:lang="en">Defines the upper tolerance limit of a parameter.</rdfs:comment>
        <rdfs:label xml:lang="en">parameter max tolerance</rdfs:label>
        <rdfs:label>parameter max tolerance</rdfs:label>
    </owl:DatatypeProperty>
    


    <!-- https://open-manufacturing.org/ontologies/I4.0/Parameter/paramMinTolerance -->


    <owl:DatatypeProperty rdf:about="https://open-manufacturing.org/ontologies/I4.0/Parameter/paramMinTolerance">
        <rdfs:domain rdf:resource="https://open-manufacturing.org/ontologies/I4.0/Parameter/Parameter"/>
        <rdfs:comment xml:lang="en">Defines the lower tolerance limit of a parameter.</rdfs:comment>
        <rdfs:label xml:lang="en">parameter min tolerance</rdfs:label>
        <rdfs:label>parameter min tolerance</rdfs:label>
    </owl:DatatypeProperty>
    


    <!-- https://open-manufacturing.org/ontologies/I4.0/Parameter/paramValue -->


    <owl:DatatypeProperty rdf:about="https://open-manufacturing.org/ontologies/I4.0/Parameter/paramValue">
        <rdfs:domain rdf:resource="https://open-manufacturing.org/ontologies/I4.0/Parameter/ParameterValue"/>
        <rdfs:comment xml:lang="en">Defines the value of a parameter.</rdfs:comment>
        <rdfs:label xml:lang="en">parameter value</rdfs:label>
        <rdfs:label>parameter value</rdfs:label>
    </owl:DatatypeProperty>
    


    <!-- 
    ///////////////////////////////////////////////////////////////////////////////////////
    //
    // Classes
    //
    ///////////////////////////////////////////////////////////////////////////////////////
     -->


    


    <!-- http://purl.oclc.org/NET/ssnx/qu/qu#Unit -->


    <owl:Class rdf:about="http://purl.oclc.org/NET/ssnx/qu/qu#Unit"/>
    


    <!-- https://open-manufacturing.org/ontologies/I4.0/Equipment/Equipment -->


    <owl:Class rdf:about="https://open-manufacturing.org/ontologies/I4.0/Equipment/Equipment">
        <rdfs:comment xml:lang="en">Generalization for all logical elements required to organize or model your manufacturing hierarchy, sequence or flow.

Note 1: The formal UML role-based equipment model object is used to define the role-based equipment hierarchy information that is defined in IEC 62264-1.

Note 2: The model contains the information that may be used to construct the hierarchical models used in manufacturing scenarios.

Reference: IEC 62264-1, IEC 62264-2</rdfs:comment>
        <rdfs:label xml:lang="en">Equipment</rdfs:label>
    </owl:Class>
    


    <!-- https://open-manufacturing.org/ontologies/I4.0/Equipment/Line -->


    <owl:Class rdf:about="https://open-manufacturing.org/ontologies/I4.0/Equipment/Line">
        <rdfs:subClassOf rdf:resource="https://open-manufacturing.org/ontologies/I4.0/Equipment/WorkCenter"/>
        <rdfs:comment xml:lang="en">Collection of one or more sequentially ordered work units that work together to perform a defined sequence of production processes to manufacture or assemble a product that can be a final or a semi-finished product. 
A line is a subclass of a work center.</rdfs:comment>
        <rdfs:label xml:lang="en">Line</rdfs:label>
    </owl:Class>
    


    <!-- https://open-manufacturing.org/ontologies/I4.0/Equipment/Plant -->


    <owl:Class rdf:about="https://open-manufacturing.org/ontologies/I4.0/Equipment/Plant">
        <rdfs:subClassOf rdf:resource="https://open-manufacturing.org/ontologies/I4.0/Equipment/Equipment"/>
        <rdfs:comment xml:lang="en">Complex and separate organizational structure set up. It is a logical grouping of a manufacturing entity. It contains other equipment such as work centers or work units. Plants may be part of business-oriented entities such as product lines, divisions, sales segments and so on.</rdfs:comment>
        <rdfs:label xml:lang="en">Plant</rdfs:label>
    </owl:Class>
    


    <!-- https://open-manufacturing.org/ontologies/I4.0/Equipment/Pool -->


    <owl:Class rdf:about="https://open-manufacturing.org/ontologies/I4.0/Equipment/Pool">
        <rdfs:subClassOf rdf:resource="https://open-manufacturing.org/ontologies/I4.0/Equipment/WorkCenter"/>
        <rdfs:comment xml:lang="en">Grouping of several parallel work units running the same process or sharing similar capabilities. 
A pool is a subclass of a work center.</rdfs:comment>
        <rdfs:label xml:lang="en">Pool</rdfs:label>
    </owl:Class>
    


    <!-- https://open-manufacturing.org/ontologies/I4.0/Equipment/Station -->


    <owl:Class rdf:about="https://open-manufacturing.org/ontologies/I4.0/Equipment/Station">
        <rdfs:subClassOf rdf:resource="https://open-manufacturing.org/ontologies/I4.0/Equipment/WorkUnit"/>
        <rdfs:comment xml:lang="en">A logical grouping of equipment intended to produce a good. Stations are often are linked to a manufacturing process for a semi-finished or finished part. Subclass of a work unit. Stations belong to a line. A line can consist of 1..n stations.

One or more process segments may be linked to a station. 

Note 1: Assets or parts within an Asset represent a station well. Station can be linked to assets via the “isImplementedBy” relationship</rdfs:comment>
        <rdfs:label xml:lang="en">Station</rdfs:label>
    </owl:Class>
    


    <!-- https://open-manufacturing.org/ontologies/I4.0/Equipment/WorkCell -->


    <owl:Class rdf:about="https://open-manufacturing.org/ontologies/I4.0/Equipment/WorkCell">
        <rdfs:subClassOf rdf:resource="https://open-manufacturing.org/ontologies/I4.0/Equipment/WorkUnit"/>
        <rdfs:comment xml:lang="en">Logical sub groupings of stations. A station can consist of 1..n work cells. Subclass of a work unit.

Work cells are intended to implement a process segment. Usually, the mapping between process segment and work cell is a 1:1 mapping.</rdfs:comment>
        <rdfs:label xml:lang="en">Work Cell</rdfs:label>
    </owl:Class>
    


    <!-- https://open-manufacturing.org/ontologies/I4.0/Equipment/WorkCenter -->


    <owl:Class rdf:about="https://open-manufacturing.org/ontologies/I4.0/Equipment/WorkCenter">
        <rdfs:subClassOf rdf:resource="https://open-manufacturing.org/ontologies/I4.0/Equipment/Equipment"/>
        <rdfs:comment xml:lang="en">Grouping of one or more work units or smaller work centers that are logically or geographically linked. Line and Pool are sub-classes of work centers. A work centers can consist of 1..n work centers (e.g., a pool is part of a line). 
This term does not refer to SAP work center. It is possible but not recommended to represent an asset as a work center.</rdfs:comment>
        <rdfs:label xml:lang="en">Work Center</rdfs:label>
    </owl:Class>
    


    <!-- https://open-manufacturing.org/ontologies/I4.0/Equipment/WorkUnit -->


    <owl:Class rdf:about="https://open-manufacturing.org/ontologies/I4.0/Equipment/WorkUnit">
        <rdfs:subClassOf rdf:resource="https://open-manufacturing.org/ontologies/I4.0/Equipment/Equipment"/>
        <rdfs:comment xml:lang="en">Logical grouping of equipment at the level below a work center. A work unit can consist of smaller work units. A work unit logically represents the location of executing a manufacturing process and can be linked to a machine or machine component which physically executes the manufacturing process.

It performs production, storage, material movement, or any other Level three or level four scheduled activity according to the manufacturing operations and control systems hierarchy.

Reference: IEC 62264-1 ID:3.1.26</rdfs:comment>
        <rdfs:label xml:lang="en">Work Unit</rdfs:label>
    </owl:Class>
    


    <!-- https://open-manufacturing.org/ontologies/I4.0/Parameter/Parameter -->


    <owl:Class rdf:about="https://open-manufacturing.org/ontologies/I4.0/Parameter/Parameter">
        <rdfs:comment xml:lang="en">An individually measured item or property of a process segment or product segment. Parameters belong to a Parameter Specification.</rdfs:comment>
        <rdfs:label xml:lang="en">Parameter</rdfs:label>
        <rdfs:label>Parameter</rdfs:label>
    </owl:Class>
    


    <!-- https://open-manufacturing.org/ontologies/I4.0/Parameter/ParameterSpecification -->


    <owl:Class rdf:about="https://open-manufacturing.org/ontologies/I4.0/Parameter/ParameterSpecification">
        <rdfs:comment xml:lang="en">Specifies the setting parameters and/or result parameters for a process segment or product segment. A parameter specification consists of 1..n parameters.</rdfs:comment>
        <rdfs:label xml:lang="en">Parameter Specification</rdfs:label>
        <rdfs:label>Parameter Specification</rdfs:label>
    </owl:Class>
    


    <!-- https://open-manufacturing.org/ontologies/I4.0/Parameter/ParameterValue -->


    <owl:Class rdf:about="https://open-manufacturing.org/ontologies/I4.0/Parameter/ParameterValue">
        <rdfs:comment xml:lang="en">Concrete value of a parameter.
Note 1: For example, the parameter value of the parameter “Temperature” might be “18.5”.</rdfs:comment>
        <rdfs:label xml:lang="en">Parameter Value</rdfs:label>
        <rdfs:label>Parameter Value</rdfs:label>
    </owl:Class>
    


    <!-- https://open-manufacturing.org/ontologies/I4.0/Parameter/ResultParameter -->


    <owl:Class rdf:about="https://open-manufacturing.org/ontologies/I4.0/Parameter/ResultParameter">
        <rdfs:subClassOf rdf:resource="https://open-manufacturing.org/ontologies/I4.0/Parameter/Parameter"/>
        <rdfs:comment xml:lang="en">Description of the result parameters of a given process or product segment. Result parameters can also contain tolerance values. Subclass of Parameter</rdfs:comment>
        <rdfs:label xml:lang="en">Result Parameter</rdfs:label>
        <rdfs:label>Result Parameter</rdfs:label>
    </owl:Class>
    


    <!-- https://open-manufacturing.org/ontologies/I4.0/Parameter/SettingParameter -->


    <owl:Class rdf:about="https://open-manufacturing.org/ontologies/I4.0/Parameter/SettingParameter">
        <rdfs:subClassOf rdf:resource="https://open-manufacturing.org/ontologies/I4.0/Parameter/Parameter"/>
        <rdfs:comment xml:lang="en">Description of input / setting parameters of a given process or product segment. Subclass of Parameter.
Note 1: Setting parameters can also contain tolerance values.</rdfs:comment>
        <rdfs:label xml:lang="en">Setting Parameter</rdfs:label>
        <rdfs:label>Setting Parameter</rdfs:label>
    </owl:Class>
    


    <!-- https://open-manufacturing.org/ontologies/I4.0/PhysicalAsset/Asset -->


    <owl:Class rdf:about="https://open-manufacturing.org/ontologies/I4.0/PhysicalAsset/Asset">
        <rdfs:comment xml:lang="en">Physical asset that covers primarily machines and tools but excludes buildings.  

Note 1: Short form asset used in this document refers to production asset.  

Assets represent an extension point. 

Note 2: You can further subclass assets (e.g. AGVs, …) 

Reference: IEC 62264-1 ID:3.1.36, Industrie 4.0 – Terms, VDI status report Industrie 4.0 (April 2021)</rdfs:comment>
        <rdfs:label xml:lang="en">Asset</rdfs:label>
    </owl:Class>
    


    <!-- https://open-manufacturing.org/ontologies/I4.0/PhysicalAsset/Building -->


    <owl:Class rdf:about="https://open-manufacturing.org/ontologies/I4.0/PhysicalAsset/Building">
        <rdfs:comment xml:lang="en">Independently usable, roofed structural works in a property. They represent a sheltered area to provide space for manufacturing assets, people and systems to perform value added activities.</rdfs:comment>
        <rdfs:label xml:lang="en">Building</rdfs:label>
    </owl:Class>
    


    <!-- https://open-manufacturing.org/ontologies/I4.0/PhysicalAsset/Level -->


    <owl:Class rdf:about="https://open-manufacturing.org/ontologies/I4.0/PhysicalAsset/Level">
        <rdfs:comment xml:lang="en">Sub-structure of a building and is synonym to the word building floor.</rdfs:comment>
        <rdfs:label xml:lang="en">Level</rdfs:label>
    </owl:Class>
    


    <!-- https://open-manufacturing.org/ontologies/I4.0/PhysicalAsset/Location -->


    <owl:Class rdf:about="https://open-manufacturing.org/ontologies/I4.0/PhysicalAsset/Location">
        <rdfs:comment>Collection of open spaces and one or more buildings on defined properties (e.g., geo fenced).
A spatial region or named place.</rdfs:comment>
        <rdfs:isDefinedBy xml:lang="en">http://purl.org/dc/terms/Location</rdfs:isDefinedBy>
        <rdfs:label xml:lang="en">Location</rdfs:label>
    </owl:Class>
    


    <!-- https://open-manufacturing.org/ontologies/I4.0/PhysicalAsset/Machine -->


    <owl:Class rdf:about="https://open-manufacturing.org/ontologies/I4.0/PhysicalAsset/Machine">
        <rdfs:subClassOf rdf:resource="https://open-manufacturing.org/ontologies/I4.0/PhysicalAsset/Asset"/>
        <rdfs:comment xml:lang="en">A specific asset (production) subclass used in manufacturing or assembly to produce tangible goods.</rdfs:comment>
        <rdfs:label xml:lang="en">Machine</rdfs:label>
    </owl:Class>
    


    <!-- https://open-manufacturing.org/ontologies/I4.0/PhysicalAsset/MachineComponent -->


    <owl:Class rdf:about="https://open-manufacturing.org/ontologies/I4.0/PhysicalAsset/MachineComponent">
        <rdfs:comment xml:lang="en">A part of a machine which itself may be composed of sub components.</rdfs:comment>
        <rdfs:label xml:lang="en">Machine Component</rdfs:label>
    </owl:Class>
    


    <!-- https://open-manufacturing.org/ontologies/I4.0/PhysicalAsset/MachineTool -->


    <owl:Class rdf:about="https://open-manufacturing.org/ontologies/I4.0/PhysicalAsset/MachineTool">
        <rdfs:comment xml:lang="en">A device used in a machine for manufacturing or assembly.  
Note 1: For example, a drilling tool is used in a drilling machine to drill holes into the product.</rdfs:comment>
        <rdfs:label xml:lang="en">Machine Tool</rdfs:label>
    </owl:Class>
    


    <!-- https://open-manufacturing.org/ontologies/I4.0/ProcessSegment/Process -->


    <owl:Class rdf:about="https://open-manufacturing.org/ontologies/I4.0/ProcessSegment/Process">
        <rdfs:comment>Description of a manufacturing process. A manufacturing process may consist of 1..n process segments</rdfs:comment>
        <rdfs:label xml:lang="en">Process</rdfs:label>
        <rdfs:label>Process</rdfs:label>
    </owl:Class>
    


    <!-- https://open-manufacturing.org/ontologies/I4.0/ProcessSegment/ProcessSegment -->


    <owl:Class rdf:about="https://open-manufacturing.org/ontologies/I4.0/ProcessSegment/ProcessSegment">
        <rdfs:comment xml:lang="en">Smallest elements of manufacturing activities that are visible to business processes. Multiple process segments together form a process (manufacturing process). Also called business process segment.</rdfs:comment>
        <rdfs:label xml:lang="en">Process Segment</rdfs:label>
        <rdfs:label>Process Segment</rdfs:label>
    </owl:Class>
    


    <!-- https://open-manufacturing.org/ontologies/I4.0/Product/Assembly -->


    <owl:Class rdf:about="https://open-manufacturing.org/ontologies/I4.0/Product/Assembly">
        <rdfs:subClassOf rdf:resource="https://open-manufacturing.org/ontologies/I4.0/Product/SemiFinishedProduct"/>
        <rdfs:comment>Description of a tangible good that is the outcome of a previous assembly process. Subclass of material. This includes especially the outcomes of other internal suppliers (e.g., plant A delivering an assembly to plant B). 
Note 1: It is a perspective of the one who uses it to build a more complex material.</rdfs:comment>
        <rdfs:label>Assembly</rdfs:label>
    </owl:Class>
    


    <!-- https://open-manufacturing.org/ontologies/I4.0/Product/Component -->


    <owl:Class rdf:about="https://open-manufacturing.org/ontologies/I4.0/Product/Component">
        <rdfs:subClassOf rdf:resource="https://open-manufacturing.org/ontologies/I4.0/Product/SemiFinishedProduct"/>
        <rdfs:comment>Description of a tangible good that is input to an assembly process and is typically purchased from a supplier in a “ready for use” form. Subclass of material.
Note 1: For example, electronic components, bolts and nuts, gear box for a car OEM. 
Note 2: It is a perspective of the one who uses it to build a more complex material.</rdfs:comment>
        <rdfs:label>Component</rdfs:label>
    </owl:Class>
    


    <!-- https://open-manufacturing.org/ontologies/I4.0/Product/Material -->


    <owl:Class rdf:about="https://open-manufacturing.org/ontologies/I4.0/Product/Material">
        <rdfs:comment>Abstraction of a tangible result of some manufacturing or assembly process. A product, semi-finished product, sub-assembly, component, or raw material. 
Note 1: The term has been purposely selected to create an umbrella for a broad spectrum of possible examples, anAbstraction of a tangible result of some manufacturing or assembly process. A product, semi-finished product, sub-assembly, component, or raw material. 
Note 2: Subclasses like product, semi-finished product and raw material allow for more precise and perspective specific classification of materials for the specific context.</rdfs:comment>
        <rdfs:label>Material</rdfs:label>
    </owl:Class>
    


    <!-- https://open-manufacturing.org/ontologies/I4.0/Product/ProcessedPart -->


    <owl:Class rdf:about="https://open-manufacturing.org/ontologies/I4.0/Product/ProcessedPart">
        <rdfs:comment>Description of a unique example/occurrence of a specific material. As such it can be an instantiation of any of the material subclasses. A processed part refers to material it represents via the “relatesToMaterial” relationship.</rdfs:comment>
        <rdfs:label>Processed Part</rdfs:label>
    </owl:Class>
    


    <!-- https://open-manufacturing.org/ontologies/I4.0/Product/Product -->


    <owl:Class rdf:about="https://open-manufacturing.org/ontologies/I4.0/Product/Product">
        <rdfs:subClassOf rdf:resource="https://open-manufacturing.org/ontologies/I4.0/Product/Material"/>
        <rdfs:comment>Description of a tangible good that is manufactured or assembled and considered ready for being sold to a customer afterwards. Subclass of material.
Note 1: Product is a perspective of the one who makes it ready for selling.</rdfs:comment>
        <rdfs:label>Product</rdfs:label>
    </owl:Class>
    


    <!-- https://open-manufacturing.org/ontologies/I4.0/Product/ProductInstance -->


    <owl:Class rdf:about="https://open-manufacturing.org/ontologies/I4.0/Product/ProductInstance">
        <rdfs:subClassOf rdf:resource="https://open-manufacturing.org/ontologies/I4.0/Product/ProcessedPart"/>
        <rdfs:comment>Concrete and unique example/occurrence of a product (definition) which is the outcome of manufacturing or assembly. A Product Instance refers to its product (definition) via the “relatesToMaterial” relationship inherited from ProcessedPart.</rdfs:comment>
        <rdfs:label>Product Instance</rdfs:label>
    </owl:Class>
    


    <!-- https://open-manufacturing.org/ontologies/I4.0/Product/RawMaterial -->


    <owl:Class rdf:about="https://open-manufacturing.org/ontologies/I4.0/Product/RawMaterial">
        <rdfs:subClassOf rdf:resource="https://open-manufacturing.org/ontologies/I4.0/Product/Material"/>
        <rdfs:comment>Description of a tangible substrate of a specific manufacturing process that is taken in its basic form as input for subsequent manufacturing. It shall not generally be used in the context of tangible input into assembly process. Subclass of material.
 Note 1: It is a perspective on the one who uses it to manufacture other goods – for example a silicon wafer is raw material for production of semi-conductor electronic devices, where by itself it is a result of complex preparation process, hence a product from perspective of its supplier.</rdfs:comment>
        <rdfs:label>Raw Material</rdfs:label>
    </owl:Class>
    


    <!-- https://open-manufacturing.org/ontologies/I4.0/Product/SemiFinishedProduct -->


    <owl:Class rdf:about="https://open-manufacturing.org/ontologies/I4.0/Product/SemiFinishedProduct">
        <rdfs:subClassOf rdf:resource="https://open-manufacturing.org/ontologies/I4.0/Product/Material"/>
        <rdfs:comment>Description of a tangible good that is not yet finished. Subclass of material.
Note 1: Usually, a semi-finished product is a sub-assembly or a component of another more complex material and is not sold to a customer by itself.</rdfs:comment>
        <rdfs:label>Semi-Finished Product</rdfs:label>
    </owl:Class>
    


    <!-- https://open-manufacturing.org/ontologies/I4.0/ProductSegment/EquipmentSpecification -->


    <owl:Class rdf:about="https://open-manufacturing.org/ontologies/I4.0/ProductSegment/EquipmentSpecification">
        <rdfs:comment xml:lang="en">Specification of the required equipment (e.g., stations, work cells) that are required to execute the product segment.</rdfs:comment>
        <rdfs:label xml:lang="en">Equipment Specification</rdfs:label>
        <rdfs:label>Equipment Specification</rdfs:label>
    </owl:Class>
    


    <!-- https://open-manufacturing.org/ontologies/I4.0/ProductSegment/MaterialSpecification -->


    <owl:Class rdf:about="https://open-manufacturing.org/ontologies/I4.0/ProductSegment/MaterialSpecification">
        <rdfs:comment xml:lang="en">Specifies the material required for executing the product segment. The material specification can refer to the input material and output material of the product segment.</rdfs:comment>
        <rdfs:label xml:lang="en">Material Specification</rdfs:label>
        <rdfs:label>Material Specification</rdfs:label>
    </owl:Class>
    


    <!-- https://open-manufacturing.org/ontologies/I4.0/ProductSegment/ProductSegment -->


    <owl:Class rdf:about="https://open-manufacturing.org/ontologies/I4.0/ProductSegment/ProductSegment">
        <rdfs:comment xml:lang="en">Implementation of a process segment for a concrete product. Thus, a product segment implements a process segment for a concrete product or product variant. A product segment identifies personnel, equipment, and material resources required of a process segment to complete a production step for a specific product. Product specific routing information between product segments can be expressed via the isFollowedBy relationship between product segments. Reference: IEC 62264-1 ID:3.1.29.</rdfs:comment>
        <rdfs:label xml:lang="en">Product Segment</rdfs:label>
        <rdfs:label>Product Segment</rdfs:label>
    </owl:Class>
    


    <!-- https://open-manufacturing.org/ontologies/I4.0/ProductSegment/SegmentResult -->


    <owl:Class rdf:about="https://open-manufacturing.org/ontologies/I4.0/ProductSegment/SegmentResult">
        <rdfs:comment xml:lang="en">Outcome of the execution of a product segment for a given product instance or processed part (see product model). A segment result refers to the parameter values of result parameters defined by the parameter specification (see Parameter Model for details).</rdfs:comment>
        <rdfs:label xml:lang="en">Segment Result</rdfs:label>
        <rdfs:label>Segment Result</rdfs:label>
    </owl:Class>
</rdf:RDF>



<!-- Generated by the OWL API (version 5.1.18) https://github.com/owlcs/owlapi/ -->


